Barebones adaptation of RISCV to MachineModule

src/Core/RISCVMachine.v
@@ -3,7 +3,7 @@ Require Import Coq.Lists.List.
 Import List.ListNotations.
 Require Import Bool.
 
-From StackSafety Require Import MachineModule PolicyModule.
+From StackSafety Require Import MachineModule (* PolicyModule *).
 
 Require Import coqutil.Word.Naive.
 Require Import coqutil.Word.Properties.
@@ -33,25 +33,26 @@ Require Import Lia.
 From RecordUpdate Require Import RecordSet.
 Import RecordSetNotations.
 
-From QuickChick Require Import QuickChick.
+(* From QuickChick Require Import QuickChick. *)
 
 Module Type RISCV <: Machine.
   Export RiscvMachine.
 
-Axiom exception : forall {A}, string -> A.
-Extract Constant exception =>
-  "(fun l ->
-   let s = Bytes.create (List.length l) in
-   let rec copy i = function
-    | [] -> s
-    | c :: l -> Bytes.set s i c; copy (i+1) l
-   in failwith (""Exception: "" ^ Bytes.to_string (copy 0 l)))".
+(* Axiom exception : forall {A}, string -> A. *)
+(* Extract Constant exception => *)
+(*   "(fun l -> *)
+(*    let s = Bytes.create (List.length l) in *)
+(*    let rec copy i = function *)
+(*     | [] -> s *)
+(*     | c :: l -> Bytes.set s i c; copy (i+1) l *)
+(*    in failwith (""Exception: "" ^ Bytes.to_string (copy 0 l)))". *)
 
   Definition Word := MachineInt.
   (* Parameter Word *)
+  Definition Addr : Type := Word.
 
-  Instance ShowWord : Show word :=
-    {| show x := show (word.signed x) |}.
+  (* Instance ShowWord : Show word := *)
+  (*   {| show x := show (word.signed x) |}. *)
 
   Definition wlt : Word -> Word -> bool := Z.ltb.
   (*  Parameter wlt : Word -> Word -> bool. *)
@@ -64,18 +65,19 @@ Extract Constant exception =>
   Lemma weq_implies_eq :
     forall w1 w2,
       weq w1 w2 = true -> w1 = w2.
+  Proof.
     apply Z.eqb_eq.
   Qed.
 
-  Lemma not_weq_implies_neq :
-    forall w1 w2,
-      weq w1 w2 = false -> w1 <> w2.
-  Proof. 
-    intros w1 w2 HEqb HEq. unfold weq in *.
-    apply Z.eqb_eq in HEq.
-    rewrite HEq in HEqb.
-    congruence.
-  Qed.
+  (* Lemma not_weq_implies_neq : *)
+  (*   forall w1 w2, *)
+  (*     weq w1 w2 = false -> w1 <> w2. *)
+  (* Proof.  *)
+  (*   intros w1 w2 HEqb HEq. unfold weq in *. *)
+  (*   apply Z.eqb_eq in HEq. *)
+  (*   rewrite HEq in HEqb. *)
+  (*   congruence. *)
+  (* Qed. *)
 
   Definition wle (w1 w2: Word) : bool :=
     orb (wlt w1 w2) (weq w1 w2).
@@ -84,73 +86,88 @@ Extract Constant exception =>
     Parameter wplus : Word -> nat -> Word.
     Parameter wminus : Word -> nat -> Word.
    *)
-  Definition wplus (w : Word) (n : nat) : Word :=
-    w + Z.of_nat n.
+  Definition wplus (w : Word) (n : Z) : Word :=
+    w + n.
 
-  Lemma wplus_neq : forall w (n : nat),
-      (n > O)%nat -> w <> wplus w n.
+  Definition wminus (w : Word) (n : Z) : Word :=
+    w - n.
+
+  Lemma wplus_neq : forall w (n : Z),
+      (n > 0)%Z -> w <> wplus w n.
   Proof.
     intros w n H Contra.
     unfold wplus in *.
     lia.
   Qed.
 
-  Definition wminus (w : Word) (n : nat) : Word :=
-    w - Z.of_nat n.
+  (* Definition wtoa (w:Word) : option Addr := Some w. *)
 
-  Definition Addr : Type := Word.
-
-  Definition wtoa (w:Word) : option Addr := Some w.
-
-  Definition alt := wlt.
-  Definition aeq := weq.
-  Definition AddrEqDec := WordEqDec.
-  Definition aeq_implies_eq := weq_implies_eq.
-  Definition not_aeq_implies_neq := not_weq_implies_neq.
-  Definition ale := wle.
-  Definition aplus := wplus.
-  Definition aplus_neq := wplus_neq.
-  Definition aminus := wminus.
+  (* Definition alt := wlt. *)
+  (* Definition aeq := weq. *)
+  (* Definition AddrEqDec := WordEqDec. *)
+  (* Definition aeq_implies_eq := weq_implies_eq. *)
+  (* Definition not_aeq_implies_neq := not_weq_implies_neq. *)
+  (* Definition ale := wle. *)
+  (* Definition aplus := wplus. *)
+  (* Definition aplus_neq := wplus_neq. *)
+  (* Definition aminus := wminus. *)
   
   Definition Register : Type := Word.
 
   Definition RA := 1.
   Definition SP := 2.
-  Definition regEq : Register -> Register -> bool := Z.eqb.
+  Definition regEqb : Register -> Register -> bool := Z.eqb.
 
-  Inductive Component:=
+  (* TODO *)
+  Definition callee_save (r : Register) : bool :=
+    match r with
+    | 1 | 2 => true
+    | _ => false
+    end.
+
+  Lemma RA_callee_save : callee_save RA = true.
+  Proof.
+    reflexivity.
+  Qed.
+
+  Lemma SP_callee_save : callee_save SP = true.
+  Proof.
+    reflexivity.
+  Qed.
+
+  Inductive Element :=
   | Mem (a:Addr)
   | Reg (r:Register)
   | PC.
 
-  Derive Show for Component.
+  (* Derive Show for Element. *)
 
-  Definition keqb (k1 k2 : Component) : bool :=
+  Definition keqb (k1 k2 : Element) : bool :=
     match k1, k2 with
     | Mem a1, Mem a2 => Z.eqb a1 a2
-    | Reg r1, Reg r2 => regEq r1 r2
+    | Reg r1, Reg r2 => regEqb r1 r2
     | PC, PC => true
     | _, _ => false
     end.
 
-  Axiom keqb_implies_eq :
-    forall k1 k2,
-      keqb k1 k2 = true -> k1 = k2.
-  Axiom not_keqb_implies_neq :
-    forall k1 k2,
-      keqb k1 k2 = false -> k1 <> k2.
+  (* Axiom keqb_implies_eq : *)
+  (*   forall k1 k2, *)
+  (*     keqb k1 k2 = true -> k1 = k2. *)
+  (* Axiom not_keqb_implies_neq : *)
+  (*   forall k1 k2, *)
+  (*     keqb k1 k2 = false -> k1 <> k2. *)
 
   (* A Value is a Word. *)
-  Definition Value : Type := Word.
-  Definition vtow (v : Value) : Word := v.
+  (* Definition Value : Type := Word. *)
+  (* Definition vtow (v : Value) : Word := v. *)
 
   (* We use a risc-v machine as our machine state and a view as a map from its
      components to their values. *)
   Definition MachineState := RiscvMachine.
-  Definition View := Component -> Value.
+  (* Definition View := Component -> Value. *)
 
   (* Project what we care about from the RiscV state. *)
-  Definition proj (m:  MachineState) (k: Component):  Value :=
+  Definition proj (m:  MachineState) (k: Element):  Word :=
     match k with
     | Mem a =>
       match (Spec.Machine.loadWord Spec.Machine.Execute (word.of_Z a)) m with
@@ -169,12 +186,12 @@ Extract Constant exception =>
       end
     end.
 
-  Definition projw := fun m k => vtow (proj m k).
+  (* Definition projw := fun m k => vtow (proj m k). *)
 
-  Lemma proj_vtow : forall m k, vtow (proj m k) = vtow (projw m k). Proof. intros;auto. Qed.
+  (* Lemma proj_vtow : forall m k, vtow (proj m k) = vtow (projw m k). Proof. intros;auto. Qed. *)
 
   (* Maybe name this pullback instead *)
-  Definition jorp (m : MachineState) (k : Component) (v : Value) : MachineState :=
+  Definition jorp (m : MachineState) (k : Element) (v : Word) : MachineState :=
     match k with
     | Mem a =>
       withMem
@@ -186,7 +203,7 @@ Extract Constant exception =>
       withPc (word.of_Z v) m
     end.
   
-  Definition getComponents (m : MachineState) : list Component :=
+  Definition getElements (m : MachineState) : list Element :=
     (* PC *)
     let pc := [PC] in
     (* Non-zero registers. *)
@@ -205,90 +222,107 @@ Extract Constant exception =>
                     (RiscvMachine.getMem m)) in
     pc ++ regs ++ mem.
 
-  Parameter ObsType : Type.
+  Parameter Event : Type.
+
+  Parameter event_eqb : Event -> Event -> bool.
 
   (* Observations are values, or silent (tau) *)
   Inductive Observation : Type := 
-  | Out (w:ObsType) 
+  | Out (w:Event)
   | Tau.
 
-  Parameter obs_eqb : Observation -> Observation -> bool.
-
-  Definition w32_eqb (w1 w2 : w32) : bool :=
-    let l1 := HList.tuple.to_list w1 in
-    let l2 := HList.tuple.to_list w2 in
-    let l12 := List.combine l1 l2 in
-    forallb (fun '(b1, b2) => Byte.eqb b1 b2) l12.
-
-  Definition memAddr_eqb (mem mem' : DefaultMemImpl32.Mem) (addr : word32) : bool :=
-    match loadWord mem addr, loadWord mem' addr with
-    | Some w, Some w' => w32_eqb w w'
+  Definition obs_eqb (o1 o2 : Observation) : bool :=
+    match o1, o2 with
+    | Out e1, Out e2 => event_eqb e1 e2
+    | Tau, Tau => true
     | _, _ => false
     end.
 
-  (* TODO: We don't have information about which parts of memory to monitor for
-     changes. On a first approximation, monitor all positions (aligned accesses
-     only) outside the code segment (whose limits are here, again for simplicity,
-     hardcoded). *)
-  Parameter findDiff : MachineState -> MachineState -> option ObsType.
+  (* Definition w32_eqb (w1 w2 : w32) : bool := *)
+  (*   let l1 := HList.tuple.to_list w1 in *)
+  (*   let l2 := HList.tuple.to_list w2 in *)
+  (*   let l12 := List.combine l1 l2 in *)
+  (*   forallb (fun '(b1, b2) => Byte.eqb b1 b2) l12. *)
 
+  (* Definition memAddr_eqb (mem mem' : DefaultMemImpl32.Mem) (addr : word32) : bool := *)
+  (*   match loadWord mem addr, loadWord mem' addr with *)
+  (*   | Some w, Some w' => w32_eqb w w' *)
+  (*   | _, _ => false *)
+  (*   end. *)
+
+  (* (* TODO: We don't have information about which parts of memory to monitor for *)
+  (*    changes. On a first approximation, monitor all positions (aligned accesses *)
+  (*    only) outside the code segment (whose limits are here, again for simplicity, *)
+  (*    hardcoded). *) *)
+  Parameter findDiff : MachineState -> MachineState -> option Event.
+
+  Definition FunID := nat.
+  (* Definition StackID := nat. *)
+
+  (* Definition EntryMap := Addr -> bool. *)
+
+  (* Definition StackMap := Addr -> option StackID. *)
+
+  (* Inductive CodeAnnotation := *)
+  (* | call *)
+  (* | retrn *)
+  (* | yield *)
+  (* | scall (f: MachineState -> Addr -> bool) *)
+  (* | normal *)
+  (* . *)
+  
+  (* Definition CodeMap := Addr -> option CodeAnnotation. *)
+
+  (* (* Stack ID of stack pointer *) *)
+  (* Definition activeStack (sm: StackMap) (m: MachineState) : *)
+  (*   option StackID := *)
+  (*   sm (proj m (Reg SP)). *)
+
+  (* Definition stack_eqb : StackID -> StackID -> bool := *)
+  (*   Nat.eqb. *)
+
+  (* Definition optstack_eqb (o1 o2 : option StackID) : bool := *)
+  (*   match o1, o2 with *)
+  (*   | Some n1, Some n2 => stack_eqb n1 n2 *)
+  (*   | None, None => true *)
+  (*   | _, _ => false *)
+  (*   end. *)
+
+  (* Definition justRet (mc m: MachineState) : Prop := *)
+  (*   proj m PC = wplus (proj mc PC) 4 /\ proj m (Reg SP) = proj mc (Reg SP). *)
+
+  (* Definition justRet_dec mc m : {justRet mc m} + {~ justRet mc m}. *)
+  (* Proof. *)
+  (*   unfold justRet. *)
+  (*   destruct (WordEqDec (proj m PC) (wplus (proj mc PC) 4)); *)
+  (*     destruct (WordEqDec (proj m (Reg SP)) (proj mc (Reg SP))); *)
+  (*     try solve [left; auto]; *)
+  (*     right; intros [? ?]; auto. *)
+  (* Qed. *)
+
+  Inductive Operation : Type :=
+  | Call (f:FunID) (reg_args:list Register) (stk_args:list (Register*Z*Z))
+  | Tailcall (f:FunID) (reg_args:list Register) (stk_args:list (Register*Z*Z))
+  | Return
+  | Alloc (off:Z) (sz:Z)
+  | Dealloc (off:Z) (sz:Z)
+  .
+
+  (* TODO: operations *)
   (* A Machine State can step to a new Machine State plus an Observation. *)
-  Definition step (m : RiscvMachine) : RiscvMachine * Observation :=
+  Definition step (m : MachineState) : MachineState * list Operation * Observation :=
     (* returns option unit * state *)
     match Run.run1 RV32IM m with
     | (_, s') =>
       if Z.eqb (word.unsigned (getPc m))
                (word.unsigned (getPc s'))
       then
-        (s', Tau)
-      else          
+        (s', [], Tau)
+      else
         match findDiff m s' with
-        | Some v => (s', Out v)
-        | None => (s', Tau)
+        | Some v => (s', [], Out v)
+        | None => (s', [], Tau)
         end
     end.
 
-  Definition FunID := nat.
-  Definition StackID := nat.
-
-  Definition EntryMap := Addr -> bool.
-
-  Definition StackMap := Addr -> option StackID.
-
-  Inductive CodeAnnotation :=
-  | call
-  | retrn
-  | yield
-  | scall (f: MachineState -> Addr -> bool)
-  | normal
-  .
-  
-  Definition CodeMap := Addr -> option CodeAnnotation.
-
-  (* Stack ID of stack pointer *)
-  Definition activeStack (sm: StackMap) (m: MachineState) :
-    option StackID :=
-    sm (proj m (Reg SP)).
-
-  Definition stack_eqb : StackID -> StackID -> bool :=
-    Nat.eqb.
-
-  Definition optstack_eqb (o1 o2 : option StackID) : bool :=
-    match o1, o2 with
-    | Some n1, Some n2 => stack_eqb n1 n2
-    | None, None => true
-    | _, _ => false
-    end.
-
-  Definition justRet (mc m: MachineState) : Prop :=
-    proj m PC = wplus (proj mc PC) 4 /\ proj m (Reg SP) = proj mc (Reg SP).
-
-  Definition justRet_dec mc m : {justRet mc m} + {~ justRet mc m}.
-  Proof.
-    unfold justRet.
-    destruct (WordEqDec (proj m PC) (wplus (proj mc PC) 4));
-      destruct (WordEqDec (proj m (Reg SP)) (proj mc (Reg SP)));
-      try solve [left; auto];
-      right; intros [? ?]; auto.
-  Qed.
 End RISCV.
